\documentclass[12pt, titlepage,french]{article}
\input{../preambule.tex}
%% -----------------------------
%% Section Font customization
%% -----------------------------
\usepackage{sectsty}
\sectionfont{\color{cobalt}}
\subsectionfont{\color{indigo(web)}}
\begin{document}
\title{Ironic proofs}
\vspace{-8ex}
\date{}
\author{Alec James van Rassel}
\maketitle

\tableofcontents
\setcounter{secnumdepth}{-1}

\clearpage

%\addcontentsline{toc}{section}{Unnumbered Section}
\section{Proof of homogeneity of the sinal function}

\begin{theorems}[Theorem]
	-\sin(x)&=	\sin(-x) 
\end{theorems}

\begin{distributions}[Proof]
\begin{enumerate}
	\item	We define:
		\begin{align*}
		sign(x)	&=	\textcolor{blue}{+}	&
		sign(-x)	&=	\textcolor{red}{-}
		\end{align*}
	\item	We apply the \textcolor{purple}{\textbf{phonetic equivalence principle}} of $\sin$ and $sign$:
		\begin{align*}
						-\sin(x)					&=	\sin(-x)	\\		
		\Leftrightarrow	-sign(x)					&=	sign(-x)		\quad	\text{\textcolor{purple}{by phonetic equivalence}}\\		
		\Leftrightarrow	-(\textcolor{blue}{+})	&=	\textcolor{red}{-}	\\		
		\Rightarrow	\textcolor{red}{-}		&=	\textcolor{red}{-}	
		\end{align*}		
	\item[$\therefore$]	$-\sin(x)=	\sin(-x)$
\end{enumerate}
\end{distributions}
$\blacksquare$

\clearpage

\section{Proof of equivalence of addition to multiplication in the definition of the factorial}

\begin{theorems}[Theorem]
	n!	
	&=	\overset{n - 1}{\underset{i = 0}{\prod}} (n - i)	
	\Leftrightarrow		\overset{n - 1}{\underset{i = 0}{\sum}} (n - i)	
\end{theorems}

\begin{distributions}[Proof]
\begin{enumerate}
	\item	It is known that:
		\begin{align*}
		n!	
		&=	\overset{n - 1}{\underset{i = 0}{\prod}} (n - i)	
		=	(n - 0) \times (n - 1) \times \dots \times 1
		\end{align*}
	\item	We apply the \textcolor{red}{\textbf{rotation property}} of multiplication
		\begin{align*}
		n!	
		=	\overset{n - 1}{\underset{i = 0}{\prod}} (n - i)	
		&=	(n - 0)\ \textcolor{black}{\times}\ (n - 1)\ \textcolor{black}{\times}\ \dots\ \textcolor{black}{\times}\ 1	\\
		&=	(n - 0)\ \textcolor{red}{\overset{\curvearrowright}{+}}\ (n - 1)\ \textcolor{red}{\overset{\curvearrowright}{+}}\ \dots\ \textcolor{red}{\overset{\curvearrowright}{+}}\ 1	\\
		&=	(n - 0)\ \textcolor{black}{+}\ (n - 1)\ \textcolor{black}{+}\ \dots\ \textcolor{black}{+}\ 1	\\
		&=	\overset{n - 1}{\underset{i = 0}{\sum}} (n - i)	
		\end{align*}		
	\item[$\therefore$]	$n!	=	\overset{n - 1}{\underset{i = 0}{\sum}} (n - i)$
\end{enumerate}
\end{distributions}

\begin{formula}{Examples of application}
\begin{minipage}{0.5\linewidth}
\begin{align*}
	3!
	&=	\overset{3 - 1}{\underset{i = 0}{\prod}} (3 - i)
	=	3 \times 2 \times 1	= 6	\\
	&\Leftrightarrow	\overset{3 - 1}{\underset{i = 0}{\sum}}
	=	3 + 2 + 1 = 6
\end{align*}
\end{minipage}
\begin{minipage}{0.5\linewidth}
\begin{align*}
	1!
	&=	\overset{1 - 1}{\underset{i = 0}{\prod}}
	=	1	\\
	&\Leftrightarrow		\overset{1 - 1}{\underset{i = 0}{\sum}} (1 - i)	
	=	1
\end{align*}
\end{minipage}
\end{formula}
$\blacksquare$

\clearpage

\section{Proof of Taylor Expansion}

\begin{distributions}[Proof]
\begin{enumerate}[label = \roman*.]
	\item	Taylor;
	\item	T\ a\ y\ l\ o\ r;
	\item	T\, a\, y\, l\, o\, r;
	\item	T\: a\: y\: l\: o\: r;
	\item	T\; a\; y\; l\; o\; r;
	\item	T\;\; a\;\; y\;\; l\;\; o\;\; r;
	\item	T\;\;\quad a\;\;\quad y\;\;\quad l\;\;\quad o\;\;\quad r;
	\item	T\;\;\quad\quad a\;\;\quad\quad y\;\;\quad\quad l\;\;\quad\quad o\;\;\quad\quad r;
	\item	T\;\;\quad\quad\quad a\;\;\quad\quad\quad y\;\;\quad\quad\quad l\;\;\quad\quad\quad o\;\;\quad\quad\quad r;
	\item	T\;\;\quad\quad\quad\quad a\;\;\quad\quad\quad\quad y\;\;\quad\quad\quad\quad l\;\;\quad\quad\quad\quad o\;\;\quad\quad\quad\quad r;
\end{enumerate}
\end{distributions}
$\blacksquare$

\clearpage

\end{document}